feat: finish basic backbone of LocalDateTime

LocalDateTimeImpl.cs
@@ -1,0 +1,24 @@
+using System;
+using System.Linq;
+using Dafny;
+
+public static class LocalDateTimeImpl
+{
+    public static ISequence<Rune> NowComponents()
+    {
+        var now = DateTime.Now;
+        var components = new[] {
+            now.Year,
+            now.Month,
+            now.Day,
+            now.Hour,
+            now.Minute,
+            now.Second,
+            now.Millisecond
+        };
+        
+        // Convert to sequence of integers as runes
+        var runes = components.Select(i => new Rune(i)).ToArray();
+        return Sequence<Rune>.FromArray(runes);
+    }
+}
