README.md
@@ -1,2 +1,11 @@
 # AWS-Dafny
 Current Design of DateTime API
+
+
+## How to execute the test example
+
+```
+dafny build --target:cs TestLocalDateTime.dfy LocalDateTimeImpl.cs
+
+./TestLocalDateTime
+```
